Setlec/SetR.lean
@@ -2,6 +2,9 @@ import Setlec.SetR.Rel
 import Setlec.SetR.AnnotOkV
 import Setlec.SetR.Sound.Motives
 import Setlec.SetR.Sound.Struct
+import Setlec.SetR.Sound.Irrel
+import Setlec.SetR.Sound.Rigidity
+import Setlec.SetR.Sound.Stuck
 import Setlec.SetR.Weaken
 import Setlec.SetR.CtxOkR
 import Setlec.SetR.Decl
